\subsection{Integration by parts}
This is equivalent to the product rule for integration. Suppose we have two function $u(x)$ and $v(x)$. Then the product rule states
\[\frac{d}{dx}(uv)=u'v+uv'.\]
Rearranging the above gives
\[uv'=\frac{d}{dx}(uv)-u'v.\]
Integrating both sides we get
\begin{eqnarray*}
\int uv'\dx &=& \int\frac{d}{dx}(uv)\dx-\int u'v\dx \\
&=& uv-\int u'v\dx.
\end{eqnarray*}
So we write the rule for integration by parts as:
\begin{thing}{Integration by Parts}
\begin{equation*}
\int u\frac{dv}{dx}\dx=uv-\int v\frac{du}{dx}\dx.
\end{equation*}
\end{thing}

\begin{example}
\[\int xe^x\dx\]
Let: 
\[u=x,\quad v'=e^x\]This means that:\[ u'=1,\quad v=e^x.\]
Therefore, we can calculate the integral as follows:
\begin{eqnarray*}
\int xe^x\dx &=& \int uv'\dx \\
&=&uv-\int u'v\dx \\
&=& xe^x-\int e^x\dx \\
&=& xe^x-e^x + c.
\end{eqnarray*}
Check:
\[\frac{d}{dx}\left[xe^x-e^x + c\right]=e^x+xe^x-e^x=xe^x.\]
\end{example}

\begin{example}
\[\int\ln x\dx\]
This is the same as
\[\int1\cdot\ln x\dx\]
We choose:
\[u=\ln x,\quad v'=1\]This means that: \[u'=\frac{1}{x},\quad v=x.\]
So we calculate the integral as
\begin{eqnarray*}
\int\ln x\dx &=& \int 1\cdot\ln x\dx \\
&=& \int uv'\dx \\
&=& uv- \int u'v\dx \\
&=& x\ln x-\int\frac{1}{x}\cdot x\dx \\
&=& x\ln x- x+c.
\end{eqnarray*}
Check:
\[\frac{d}{dx}\left[x\ln x- x+c\right]=\ln x+x\cdot\frac{1}{x}-1=\ln x.\]
\end{example}

\begin{example}
\[\int e^x\cos x\dx\]
Let:
\[u=\cos x,\quad v'=e^x\]This means that\[u'=-\sin x,\quad v=e^x\]
So we write our integral as
\begin{eqnarray*}
\int e^x\cos x\dx &=& \int uv'\dx\\
&=& uv-\int u'v\dx \\
&=& e^x\cos x + \int e^x\sin x\dx.
\end{eqnarray*}
Now, we have an integral similar to what we started with, so let us integrate this by parts too, choosing
\[\bar{u}=\sin x,\quad \bar{v}'=e^x \quad\quad\quad\quad \bar{u}'=\cos x,\quad \bar{v}=e^x.\]
So our original integral becomes
\begin{eqnarray*}
\int e^x\cos x\dx &=&e^x\cos x + \int \bar{u}\bar{v}'\dx\\
&=&e^x\cos x +\bar{u}\bar{v}-\int\bar{u}'\bar{v}\dx \\
&=& e^x\cos x+ e^x\sin x-\int e^x\cos x\dx.
\end{eqnarray*}
Note, now on the RHS we have the same integral we started with. Rearranging this, we can make the integral the subject:
\[\int e^x\cos x\dx  = e^x\cos x+ e^x\sin x-\int e^x\cos x\dx,\]
\[\therefore \quad 2\int e^x\cos x\dx  = e^x\cos x+ e^x\sin x.\]
So finally, we can write:
\[\int e^x\cos x\dx  = \frac{1}{2}\left[ e^x\left(\cos x+ \sin x\right)\right] + c,\]
Check:
\[\frac{d}{dx}\left[\frac{1}{2}\left[ e^x\left(\cos x+ \sin x\right)\right] + c \right] =\frac{1}{2}\left\{e^x(\cos x+\sin x)+e^x(-\sin x+\cos x)\right\}=e^x\cos x \]
\end{example}


