\subsection{Partial fractions}

We can sometimes split polynomial fractions into smaller parts.
\begin{example}
\[\frac{1}{x^2-1}\]
First factorise the denominator:
\[x^2-1 = (x+1)(x-1)\]
Now write:
\[\frac{1}{x^2-1}=\frac{A}{x-1}+\frac{B}{x+1},\]
where $A$ and $B$ are constants to be found. Multiplying everything by $(x-1)(x+1)$ gives:
\[1=A(x+1)+B(x-1)\]
Substituting in \(x=1\) gives \[1=2A.\]
Substituting in \(x=-1\) gives \[1=-2B.\]

Therefore,
\begin{eqnarray*}
A&=&\frac{1}{2}, \\
B&=&-\frac{1}{2}.
\end{eqnarray*}
Hence:
\[\frac{1}{x^2-1}=\frac{1}{2(x-1)}-\frac{1}{2(x+1)}\]
\end{example}

\begin{definition}
Splitting the fraction as above is called splitting into \textbf{partial fractions}.
\end{definition}

We can use partial fractions for integration:

\begin{example}
\begin{eqnarray*}
\int \frac{1}{x^2-1}\dx&=&\frac{1}{2}\int\frac{1}{x-1}\dx-\frac{1}{2}\int\frac{1}{x+1}\dx \\
&=&\frac{1}{2}\ln|x-1|-\frac{1}{2}\ln|x+1|+c \\
&=&\frac{1}{2}\ln\left|\frac{x-1}{x+1}\right|+c.
\end{eqnarray*}
\end{example}

\begin{example}
Consider the integral
\[\int \frac{x^2+6x+1}{3x^2+5x-2}\dx.\]
To split into partial fractions, the numerator needs to be of a lower degree than the denominator. So we manipulate as follows:
\begin{eqnarray*}
\frac{x^2+6x+1}{3x^2+5x-2}&=&\frac{\frac{1}{3}(3x^2+18x+3)}{3x^2+5x-2} \\
&=&\frac{\frac{1}{3}(3x^2+5x-2+13x+5)}{3x^2+5x-2} \\
&=&\frac{1}{3}\left[1+\frac{13x+5}{3x^2+5x-2}\right].
\end{eqnarray*}

Now we factorise the denominator:\[3x^2+5x-2=(3x-1)(x+2)\] 

Next we write split the fraction into partial fractions
\[\frac{13x+5}{3x^2+5x-2}=\frac{A}{3x-1}+\frac{B}{x+2}=\frac{(A+3B)x+2A-B}{(3x-1)(x+2)}.\]
Matching the coefficients on the numerator we must have
\begin{align*}
    \left. \begin{array}{l}
        A+3B=13  \\
        2A-B=5 
    \end{array}\right.
\end{align*}
Solving simultaeneously we have the solution $A=4$ and $B=3$. So the integral becomes

\begin{eqnarray*}
\int \frac{x^2+6x+1}{3x^2+5x-2}\dx &=& \frac{1}{2}\int 1+\frac{13x+5}{3x^2+5x-2}\dx\\
&=& \frac{1}{3}\int\dx+\frac{1}{3}\int\frac{4}{3x-1}\dx+\frac{1}{3}\int\frac{3}{x+2}\dx \\
&=& \frac{1}{3}x+\frac{4}{9}\ln|3x-1|+\ln|x+2|+c.
\end{eqnarray*}
\end{example}
