\subsubsection{$p$ is an exponential function}
If $p$ is an exponential function then we guess that the particular integral will be an exponential function.
\begin{example}
Find the general solution of the following differential equation,
\[y''+4y'+3y=5e^{4x}.\]
The auxiliary equation is
\[\lambda^2+4\lambda+3=0\quad\iff\quad(\lambda+1)(\lambda+3)=0.\]
Hence, this has two distinct real roots, namely $\lambda_1=-1$, $\lambda_2=-3$. So the C.F. (from the homogeneous equation) is given by
\[g(x)=c_1e^{-x}+c_2e^{-3x}.\]
To find the P.I. we try
\[f=ae^{4x},\]
since $p(x)=5e^4x$. Differentiating, we have
\[f'=4a^{4x},\quad f''=16a^{4x}.\]
Substituting into the differential equation we see that
\begin{align*}
f''+4f'+3f&=16ae^{4x}+16ae^{4x}+3ae^{4x}\\
&=35ae^{4x}\\
&=35ae^{4x}&\equiv 5e^{4x}.
\end{align*}
Therefore we have $a=1/7$ and so the P.I. is
\[f=\frac17e^{4x}.\]
Finally, the general solution is
\[y(x)=\frac17e^{4x}+c_1e^{-x}+c_2e^{-3x}.\]
\end{example}

\begin{example}
Solve the initial-value problem given by
\[y''+4y'+3y=e^{-x},\quad y(0)=0,\quad y'(0)=0.\]
We know from the example above that the C.F. is 
\[c_1e^{-x}+c_2e^{-3x},\]

Now let us find the P.I., if we try $f=ae^{-x}$, we know that it wouldn't work since $ae^{-x}$ is actually a solution to the homogeneous equation $y''+4y'+3y=0$. Therefore, we try 
\[f=axe^{-x},\]
thus
\[f'=ae^{-x}-axe^{-x},\quad \text{and}\quad f''=-2ae^{-x}+axe^{-x}.\]
Substituting into the differential equation we have
\begin{align*}
f''+4f'+3f &= -2ae^{-x}+axe^{-x}+4ae^{-x}-4axe^{-x}+3axe^{-x} \\
&= 2ae^{-x}\\
&\equiv e^{-x}.
\end{align*}
Therefore we must have $a=1/2$ and so the general solution to the differential equations is
\[y(x)=\frac{1}{2}xe^{-x}+c_1e^{-x}+c_2e^{-3x}.\]
Differentiating the general solution we have
\[y'(x)=\frac{1}{2}e^{-x}-\frac{1}{2}xe^{-x}-c_1e^{-x}-3c_2e^{-3x}.\]
Putting $x=0$, we have (from the initial conditions)
\begin{align*}
    \left. \begin{array}{l}
	y(0)=c_1+c_2=0 \\
	y'(0)=\frac{1}{2}-c_1-3c_2=0
    \end{array}\right\}
    \quad \implies \quad
        \left. \begin{array}{l}
	c_1=-\frac{1}{4} \\
	c_2=\frac{1}{4}
    \end{array}\right.,
\end{align*}
thus
\[y(x)=\frac{1}{2}xe^{-x}-\frac{1}{4}e^{-x}+\frac{1}{4}e^{-3x},\]
is the solution to the initial-value problem.
\end{example}

\begin{example}
Find the general solution to the equation
\[y''+2y'+y=2e^{-x}.\]

\underline{Find the C.F.}: The auxiliary equation is
\begin{align*}
\lambda^2+2\lambda+1&=0\\
(\lambda+1)^2&=0\\
\lambda_1&=-1
\end{align*}

We have a repeated root so
\[g(x)=c_1e^{-x}+c_2xe^{-x}.\]
Here $e^{-x}$ and $xe^{-x}$ are two independent solutions to the homogeneous equation
\[y''+2y'+y=0.\]

\underline{Find a P.I.}: We have to try 
\[f=ax^2e^{-x},\]
since $e^{-x}$ and $xe^{-x}$ can't be the solution to the original differential equation as they satisfy the homogeneous equation.
The derivatives are:
\begin{align*}
f'&=2axe^{-x}-ax^2e^{-x}\\\\
f''&=2ae^{-x}-2axe^{-x}-2axe^{-x}+ax^2 e^{-x}\\&=axe^{-x}-4axe^{-x}+2ae^{-x}\end{align*}
Substituting $y=f(x)$ into the differential equation, we have:
\begin{align*}
f''+2f'+f &= ax^2e^{-x}-4axe^{-x}+2ae^{-x}+4axe^{-x}-2ax^2e^{-x}+ax^2e^{-x} \\
&=2ae^{-x} \\
2ae^{-x}&\equiv 2e^{-x}
\end{align*}
Therefore $a=1$. So finally, we have the general solution
\[y(x)=(c_1+c_2x+x^2)e^{-x}.\]
\end{example}
